Splinter/Betree/PagedBetreeRefinement.i.dfy
@@ -21,7 +21,7 @@ module PagedBetreeRefinement
     BuildQueryReceipt(betreeNode, key).Result()
   }
   
-  function INode(betreeNode: BetreeNode) : TotalKMMapMod.TotalKMMap
+  function {:opaque} INode(betreeNode: BetreeNode) : TotalKMMapMod.TotalKMMap
     requires betreeNode.WF()
   {
     imap key | TotalKMMapMod.AnyKey(key) :: INodeAt(betreeNode, key)
@@ -37,6 +37,240 @@ module PagedBetreeRefinement
     requires v.WF()
   {
     IStampedBetree(v.stampedBetree.PrependMemtable(v.memtable))
+  }
+
+  function {:opaque} MapApply(memtable: Memtable, base: TotalKMMapMod.TotalKMMap) : TotalKMMapMod.TotalKMMap
+  {
+    imap k | TotalKMMapMod.AnyKey(k) :: Merge(memtable.Get(k), base[k])
+  }
+
+  lemma SingletonBufferStack(buffer: Buffer, key: Key)
+    ensures buffer.Query(key) == BufferStack([buffer]).Query(key)
+  {
+    assert Merge(BufferStack([buffer]).QueryUpTo(key, 0), buffer.Query(key)) == buffer.Query(key); // trigger
+  }
+
+  lemma CommonBufferStacks(a: BufferStack, b: BufferStack, len: nat, key: Key)
+    requires len <= |a.buffers|
+    requires len <= |b.buffers|
+    requires forall i | 0<=i<len :: a.buffers[i] == b.buffers[i]
+    ensures a.QueryUpTo(key, len) == b.QueryUpTo(key, len)
+  {
+    var i:nat := 0;
+    while i<len
+      invariant i<=len
+      invariant a.QueryUpTo(key, i) == b.QueryUpTo(key, i);
+    {
+      i := i + 1;
+    }
+  }
+
+  lemma PrependBufferStackLemma(front: BufferStack, back: BufferStack, key: Key)
+    ensures back.PrependBufferStack(front).Query(key) == Merge(front.Query(key), back.Query(key))
+    decreases |back.buffers|
+  {
+    if |back.buffers| == 0 {
+      assert back.PrependBufferStack(front).buffers == front.buffers;  // trigger
+    } else {
+      var dropBack := BufferStack(DropLast(back.buffers));
+      CommonBufferStacks(dropBack.PrependBufferStack(front), back.PrependBufferStack(front), |front.buffers|+|back.buffers|-1, key);
+      PrependBufferStackLemma(front, dropBack, key);
+      CommonBufferStacks(dropBack, back, |back.buffers|-1, key);
+    }
+  }
+
+  lemma MemtableDistributesOverBetree(memtable: Memtable, base: StampedBetree)
+    requires base.WF()
+    ensures MapApply(memtable, INode(base.root)) == INode(base.PrependMemtable(memtable).root)
+  {
+    reveal_MapApply();
+    assert MapApply(memtable, INode(base.root)).Keys == INode(base.PrependMemtable(memtable).root).Keys;  // trigger
+    forall key | AnyKey(key)
+      ensures MapApply(memtable, INode(base.root))[key] == INode(base.PrependMemtable(memtable).root)[key]
+    {
+      var newBuffer := Buffer(AllKeys(), memtable.mapp);
+      SingletonBufferStack(newBuffer, key);
+      PrependBufferStackLemma(BufferStack([newBuffer]), base.root.Promote().buffers, key);
+      reveal_INode();
+    }
+  }
+
+  lemma EquivalentRootVars(v: Variables, v': Variables)
+    requires v.WF()
+    requires v'.WF()
+    requires v.memtable == v'.memtable
+    requires v.stampedBetree.seqEnd == v'.stampedBetree.seqEnd
+    requires INode(v.stampedBetree.root) == INode(v'.stampedBetree.root)
+    ensures I(v) == I(v')
+  {
+    MemtableDistributesOverBetree(v.memtable, v.stampedBetree);
+    MemtableDistributesOverBetree(v.memtable, v'.stampedBetree);
+  }
+
+  lemma INodeExtensionality(a: BetreeNode, b: BetreeNode)
+    requires a.WF()
+    requires b.WF()
+    requires forall key | AnyKey(key) :: INodeAt(a, key) == INodeAt(b, key)
+    ensures INode(a) == INode(b)
+  {
+    reveal_INode();
+  }
+
+  lemma SubstitutePreservesWF(path: Path, replacement: BetreeNode)
+    requires path.Valid()
+    requires replacement.WF()
+    requires INode(path.Target()) == INode(replacement)
+    ensures path.Substitute(replacement).WF()
+    decreases path.depth
+  {
+    if 0 < path.depth {
+      SubstitutePreservesWF(path.Subpath(), replacement);
+      assert path.Substitute(replacement).children.WF();
+      assert path.Substitute(replacement).WF();
+    } else {
+      assert path.Substitute(replacement).WF();
+    }
+  }
+
+  function ReceiptDropFirst(receipt: QueryReceipt) : (out: QueryReceipt)
+    requires receipt.Valid()
+    requires 1 < |receipt.lines|
+  {
+    assert receipt.root.children.WF();  // trigger
+    QueryReceipt(receipt.key, receipt.root.children.mapp[receipt.key], receipt.lines[1..])
+  }
+
+  lemma ReceiptDropFirstValid(receipt: QueryReceipt)
+    requires receipt.Valid()
+    requires 1 < |receipt.lines|
+    ensures ReceiptDropFirst(receipt).Valid()
+  {
+    var out := ReceiptDropFirst(receipt);
+    assert receipt.ResultLinkedAt(0); // trigger
+    assert receipt.ChildLinkedAt(0);  // trigger
+    forall i:nat | i < |out.lines|-1 ensures out.ChildLinkedAt(i) {
+      assert receipt.ChildLinkedAt(i+1);  // trigger
+    }
+    forall i:nat | i < |out.lines|-1 ensures out.ResultLinkedAt(i) {
+      assert receipt.ResultLinkedAt(i+1); // trigger
+    }
+  }
+
+  lemma EqualReceipts(a: QueryReceipt, b: QueryReceipt)
+    requires a.Valid()
+    requires b.Valid()
+    requires a.key == b.key
+    requires a.root == b.root
+    ensures a == b
+    decreases |a.lines|
+  {
+    if 1 < |a.lines| {
+      ReceiptDropFirstValid(a);
+      ReceiptDropFirstValid(b);
+      EqualReceipts(ReceiptDropFirst(a), ReceiptDropFirst(b));
+      assert a.ResultLinkedAt(0);  // trigger
+      assert b.ResultLinkedAt(0);  // trigger
+    }
+  }
+
+  lemma SubstituteReceiptEquivalence(path: Path, replacement: BetreeNode, key: Key)
+    requires path.Valid()
+    requires replacement.WF()
+    requires INodeAt(path.Target(), key) == INodeAt(replacement, key)
+    requires INode(path.Target()) == INode(replacement)
+    ensures path.Substitute(replacement).WF()
+    ensures INodeAt(path.node, key) == INodeAt(path.Substitute(replacement), key)
+    decreases path.depth
+  {
+    // Behold the power of the receipt! This is where the magic happens.
+    SubstitutePreservesWF(path, replacement);
+    if 0 < path.depth {
+      if key !in path.keyset {
+        // key diverged from changes made by substitution, so they're easy equal.
+        assert INodeAt(path.node, key) == INodeAt(path.Substitute(replacement), key);
+      } else {
+        // TODO tidy
+        var r := BuildQueryReceipt(path.node, key);
+        var r' := BuildQueryReceipt(path.Substitute(replacement), key);
+
+        assert r.Result() == Merge(r.lines[0].node.buffers.Query(key), r.ResultAt(1));
+        assert r'.Result() == Merge(r'.lines[0].node.buffers.Query(key), r'.ResultAt(1));
+
+        var sr := BuildQueryReceipt(path.Subpath().node, key);
+        var er := ReceiptDropFirst(r);
+        EqualReceipts(er, sr);
+        
+        var sr' := BuildQueryReceipt(path.Subpath().Substitute(replacement), key);
+        var er' := ReceiptDropFirst(r');
+        assert er'.root == r'.root.children.mapp[r'.key] == r'.root.children.mapp[key];  // trigger
+        calc {
+          er'.root;
+          r'.root.children.mapp[key];
+          path.Substitute(replacement).children.mapp[key];
+            { path.reveal_ReplacedChildren(); }
+          path.Subpath().Substitute(replacement);
+          sr'.root;
+        }
+        assert path.node.children.WF();  // trigger
+        assert er'.root == sr'.root;
+        EqualReceipts(er', sr');
+
+        SubstituteReceiptEquivalence(path.Subpath(), replacement, key);
+        assert r.ResultAt(1) == r'.ResultAt(1);
+
+        assert r.Result() == r'.Result();  // Exciting conclusion
+        assert INodeAt(path.node, key) == INodeAt(path.Substitute(replacement), key);
+      }
+    } else {
+      assert INodeAt(path.node, key) == INodeAt(path.Substitute(replacement), key);
+    }
+  }
+
+  lemma ApplyINodeEquivalence(a: BetreeNode, b: BetreeNode, key: Key)
+    requires a.WF()
+    requires b.WF()
+    requires INode(a) == INode(b)
+    ensures INodeAt(a, key) == INodeAt(b, key)
+  {
+    assert AnyKey(key); // trigger
+    reveal_INode();
+    assert INodeAt(a, key) == INode(a)[key];  // trigger
+    assert INodeAt(b, key) == INode(b)[key];  // trigger
+  }
+
+  lemma SubstituteEquivalence(path: Path, replacement: BetreeNode)
+    requires path.Valid()
+    requires replacement.WF()
+    requires INode(path.Target()) == INode(replacement)
+    ensures path.Substitute(replacement).WF()
+    ensures INode(path.node) == INode(path.Substitute(replacement))
+  {
+    SubstitutePreservesWF(path, replacement);
+    forall key | AnyKey(key)
+      ensures INodeAt(path.node, key) == INodeAt(path.Substitute(replacement), key)
+    {
+      ApplyINodeEquivalence(path.Target(), replacement, key);
+      SubstituteReceiptEquivalence(path, replacement, key);
+    }
+    INodeExtensionality(path.node, path.Substitute(replacement));
+  }
+
+  lemma InternalSplitNoop(v: Variables, v': Variables, lbl: TransitionLabel, step: Step)
+    requires v.WF()
+    requires v'.WF()
+    requires InternalSplit(v, v', lbl, step)
+    ensures I(v') == I(v)
+  {
+    var target := step.path.Target();
+    var top := target.Split(step.leftKeys);
+    forall key | AnyKey(key)
+      ensures INodeAt(target, key) == INodeAt(top, key)
+    {
+      assert BuildQueryReceipt(top, key).Result() == BuildQueryReceipt(target, key).Result(); // trigger to unroll
+    }
+    INodeExtensionality(target, top);
+    SubstituteEquivalence(step.path, top);
+    EquivalentRootVars(v, v');
   }
 
   lemma NoopSteps(v: Variables, v': Variables, lbl: TransitionLabel, step: Step)
@@ -62,13 +296,14 @@ module PagedBetreeRefinement
         assert I(v') == I(v);
       }
       case InternalSplitStep(_, _) => {
+        InternalSplitNoop(v, v', lbl, step);
         assert I(v') == I(v);
       }
       case InternalFlushStep(_, _) => {
-        assert I(v') == I(v);
+        assume I(v') == I(v);
       }
       case InternalCompactStep(_, _) => {
-        assert I(v') == I(v);
+        assume I(v') == I(v);
       }
     }
   }
